Make the instantiation of the stream functor for blake2 generic in the alg and the field spec

code/streaming/Hacl.Streaming.Blake2.fst
@@ -1,4 +1,4 @@
-module Hacl.Streaming.Blake2s_32
+module Hacl.Streaming.Blake2
 
 module HS = FStar.HyperStack
 module B = LowStar.Buffer
@@ -46,12 +46,6 @@ module Incr = Spec.Hash.Incremental
 let add_zero_left_is_same (n : int) :
   Lemma(0 + n = n) = ()
 
-inline_for_extraction noextract
-let a = Spec.Blake2S
-
-inline_for_extraction noextract
-let m = M32
-
 let to_hash_alg (a : Spec.alg) =
   match a with
   | Spec.Blake2S -> Hash.Blake2S
@@ -59,44 +53,48 @@ let to_hash_alg (a : Spec.alg) =
 
 let index = unit
 
+let alg = Spec.alg
+
+let m_spec = Core.m_spec
+
 /// The stateful state: (wv, hash)
 inline_for_extraction noextract
-let s = state_p a m & state_p a m
+let s (a : alg) (m : m_spec) = state_p a m & state_p a m
 
 inline_for_extraction noextract
 let extra_state_zero_element a : Hash.extra_state (to_hash_alg a) =
   Hash.nat_to_extra_state (to_hash_alg a) 0
 
 inline_for_extraction noextract
-let t = Hash.words_state' (to_hash_alg a)
+let t (a : alg) = Hash.words_state' (to_hash_alg a)
 
 inline_for_extraction noextract
-let get_wv (s : s) : Tot (state_p a m) =
+let get_wv (#a : alg) (#m : m_spec) (s : s a m) : Tot (state_p a m) =
   match s with wv, _ -> wv
 
 inline_for_extraction noextract
-let get_state_p (s : s) : Tot (state_p a m) =
+let get_state_p (#a : alg) (#m : m_spec) (s : s a m) : Tot (state_p a m) =
   match s with _, p -> p
 
 inline_for_extraction noextract
-let state_v (h : HS.mem) (s : s) : GTot (Spec.state a) =
+let state_v (#a : alg) (#m : m_spec) (h : HS.mem) (s : s a m) : GTot (Spec.state a) =
   Core.state_v h (get_state_p s)
 
 inline_for_extraction noextract
-let s_v (h : HS.mem) (s : s) : GTot t =
+let s_v (#a : alg) (#m : m_spec) (h : HS.mem) (s : s a m) : GTot (t a) =
   state_v h s
 
 /// Small helper which facilitates inferencing implicit arguments for buffer
 /// operations
 inline_for_extraction noextract
-let state_to_lbuffer (s : state_p a m) :
+let state_to_lbuffer (#a : alg) (#m : m_spec) (s : state_p a m) :
   B.lbuffer (element_t a m) (4 * U32.v (row_len a m)) =
   s
 
 inline_for_extraction noextract
-let stateful_blake2s_32: I.stateful unit =
+let stateful_blake2 (a : alg) (m : m_spec) : I.stateful unit =
   I.Stateful
-    (fun () -> s) (* s *)
+    (fun () -> s a m) (* s *)
     (* footprint *)
     (fun #_ _ acc ->
       let wv, b = acc in
@@ -114,7 +112,7 @@ let stateful_blake2s_32: I.stateful unit =
       B.live h (state_to_lbuffer wv) /\
       B.live h (state_to_lbuffer b) /\
       B.disjoint (state_to_lbuffer wv) (state_to_lbuffer b))
-    (fun () -> t) (* t *)
+    (fun () -> t a) (* t *)
     (fun () h acc -> s_v h acc) (* v *)
     (fun #_ h acc -> let wv, b = acc in ()) (* invariant_loc_in_footprint *)
     (fun #_ l acc h0 h1 -> let wv, b = acc in ()) (* frame_invariant *)
@@ -142,121 +140,122 @@ let stateful_blake2s_32: I.stateful unit =
              U32.(4ul *^ row_len a m))
 
 inline_for_extraction noextract
-let key_size_ty = key_size:nat{0 < key_size /\ key_size <= Spec.max_key a}
+let key_size_ty (a : alg) = key_size:nat{0 < key_size /\ key_size <= Spec.max_key a}
 
 inline_for_extraction noextract
-let key_size_t = key_size:U32.t{0 < U32.v key_size /\ U32.v key_size <= Spec.max_key a}
+let key_size_t (a : alg) = key_size:U32.t{0 < U32.v key_size /\ U32.v key_size <= Spec.max_key a}
 
 inline_for_extraction noextract
-let k (key_len : key_size_t) =
+let k (#a : alg) (key_len : key_size_t a) =
   I.stateful_buffer uint8 key_len (Lib.IntTypes.u8 0)
 
-let max_input_length (key_size : nat) : nat =
-  if key_size = 0 then Spec.max_limb a
-  else Spec.max_limb a - Spec.size_block a
+/// The functor currently limits the size of the data, so we can't go as far
+/// as blake2 can go
+let max_input_length (a : alg) (key_size : nat) : nat =
+  if key_size = 0 then Spec.max_limb Spec.Blake2S
+  else Spec.max_limb Spec.Blake2S - Spec.size_block a
 
 inline_for_extraction noextract
-let block = (block: S.seq uint8 { S.length block = Spec.size_block a })
+let block (a : alg) = (block: S.seq uint8 { S.length block = Spec.size_block a })
 
 inline_for_extraction noextract
-let block_len = Core.size_block a
-
-//inline_for_extraction noextract
-//let key_size : nat = Spec.max_key a
+let block_len (a : alg) : U32.t = Core.size_block a
 
 inline_for_extraction noextract
-let key_len (key_size : key_size_ty) : U32.t = U32.uint_to_t key_size
+let output_size (a : alg) : nat = Spec.max_output a
 
 inline_for_extraction noextract
-let output_size : nat = Spec.max_output a
-
-inline_for_extraction noextract
-let output_len = U32.uint_to_t output_size
+let output_len (a : alg) = U32.uint_to_t (output_size a)
 
 /// The prevlen parameter computed by the streaming functor and given to ``update_multi``
 /// or ``update_last`` is equal to the length of the data processed so far (without the
 /// key). In the case of blake2, however, we also need to count the key (if it is not
 /// an empty seq) in the total length of processed data.
 inline_for_extraction noextract
-let blake2_prevlength (key_size : nat) (prevlen : nat) : nat =
+let blake2_prevlength (a : alg) (key_size : nat) (prevlen : nat) : nat =
   if key_size = 0 then prevlen else prevlen + Spec.size_block a
 
-let blake2_prevlength_add_right_eq (key_size : nat) (prevlen len : nat) :
+let blake2_prevlength_add_right_eq (a : alg) (key_size : nat) (prevlen len : nat) :
   Lemma(
-    blake2_prevlength key_size prevlen + len = blake2_prevlength key_size (prevlen + len))
+    blake2_prevlength a key_size prevlen + len = blake2_prevlength a key_size (prevlen + len))
   = ()
 
 /// Same function as above but with low-level types
 inline_for_extraction noextract
-let blake2_prevlen_ (key_len : U32.t)
-                    (prevlen : U64.t{ U64.v prevlen <= max_input_length (U32.v key_len) }) :
-  x:U64.t { U64.v x = blake2_prevlength (U32.v key_len) (U64.v prevlen) } =
+let blake2_prevlen_ (a : alg) (key_len : U32.t)
+                    (prevlen : U64.t { U64.v prevlen <= max_input_length a (U32.v key_len) }) :
+  x:U64.t  { U64.v x = blake2_prevlength a (U32.v key_len) (U64.v prevlen) } =
   if U32.(key_len =^ 0ul) then prevlen
-  else U64.(prevlen +^ FStar.Int.Cast.uint32_to_uint64 block_len)
+  else U64.(prevlen +^ FStar.Int.Cast.uint32_to_uint64 (block_len a))
 
 inline_for_extraction noextract
-let blake2_prevlen (key_len : U32.t)
-                   (prevlen : U64.t{ U64.v prevlen <= max_input_length (U32.v key_len) }) :
+let blake2_prevlen (a : alg) (key_len : U32.t)
+                   (prevlen : U64.t{ U64.v prevlen <= max_input_length a (U32.v key_len) }) :
   x:Spec.limb_t a {
-    Lib.IntTypes.uint_v x = blake2_prevlength (U32.v key_len) (U64.v prevlen) } =
+    Lib.IntTypes.uint_v x = blake2_prevlength a (U32.v key_len) (U64.v prevlen) } =
   let open Lib.IntTypes in
   match a with
-  | Spec.Blake2S -> to_u64 #U64 #PUB (blake2_prevlen_ key_len prevlen)
-  | Spec.Blake2B -> FStar.Int.Cast.Full.uint64_to_uint128
-                     (to_u64 #U64 #PUB (blake2_prevlen_ key_len prevlen))
+  | Spec.Blake2S -> to_u64 #U64 #PUB (blake2_prevlen_ a key_len prevlen)
+  | Spec.Blake2B ->
+    [@inline_let] let x : uint64 = to_u64 #U64 #PUB (blake2_prevlen_ a key_len prevlen) in
+    Lib.IntTypes.cast U128 SEC x
 
-let init_s (#key_size : key_size_ty) () (key : Seq.lseq uint8 key_size) : Tot t =
-  Spec.blake2_init a key_size key output_size
+let init_s (#a : alg) (#key_size : key_size_ty a) ()
+           (key : Seq.lseq uint8 key_size) : Tot (t a) =
+  Spec.blake2_init a key_size key (output_size a)
 
-let update_multi_s (key_size : key_size_ty) () (acc : t)
+let update_multi_s (#a : alg) (key_size : key_size_ty a) () (acc : t a)
                    (prevlen : nat{prevlen % Spec.size_block a = 0})
-                   (input : Seq.seq uint8{ prevlen + S.length input <= max_input_length key_size /\
+                   (input : Seq.seq uint8{ prevlen + S.length input <= max_input_length a key_size /\
                                            S.length input % Spec.size_block a = 0 }) :
-  Tot t =
-  let es = Hash.nat_to_extra_state (to_hash_alg a) (blake2_prevlength key_size prevlen) in
+  Tot (t a) =
+  let es = Hash.nat_to_extra_state (to_hash_alg a) (blake2_prevlength a key_size prevlen) in
   let s = (acc, es) in
   fst (Agile.update_multi (to_hash_alg a) s input)
 
-let update_last_s (key_size : key_size_ty) () (acc : t)
+let update_last_s (#a : alg) (key_size : key_size_ty a) () (acc : t a)
                   (prevlen : nat{prevlen % Spec.size_block a = 0})
-                  (input : Seq.seq uint8{ S.length input + prevlen <= max_input_length key_size /\
+                  (input : Seq.seq uint8{ S.length input + prevlen <= max_input_length a key_size /\
                                           S.length input <= Spec.size_block a }) :
-  Tot t =
-  let es = Hash.nat_to_extra_state (to_hash_alg a) (blake2_prevlength key_size prevlen) in
+  Tot (t a) =
+  let es = Hash.nat_to_extra_state (to_hash_alg a) (blake2_prevlength a key_size prevlen) in
   let s = (acc, es) in
   fst (Spec.Hash.Incremental.update_last (to_hash_alg a) s prevlen input)
 
-let finish_s (#key_size : key_size_ty) () (key : S.seq uint8{S.length key = key_size}) (acc : t) :
-  output : S.seq uint8 { S.length output = U32.v output_len } =
+let finish_s (#a : alg) (#key_size : key_size_ty a) ()
+             (key : S.seq uint8{S.length key = key_size}) (acc : t a) :
+  output : S.seq uint8 { S.length output = U32.v (output_len a) } =
   (* The extra state is actually not used, so we initialize it to a dummy value *)
   let s = (acc, Hash.nat_to_extra_state (to_hash_alg a) 0) in
   Spec.Hash.PadFinish.finish (to_hash_alg a) s
 
-let spec_s (#key_size : key_size_ty) ()
+let spec_s (a : alg) (#key_size : key_size_ty a) ()
            (key : S.seq uint8{S.length key = key_size})
-           (input : S.seq uint8{S.length input <= max_input_length key_size}) = 
-  Spec.blake2 a input key_size key output_size
+           (input : S.seq uint8{S.length input <= max_input_length a key_size}) = 
+  Spec.blake2 a input key_size key (output_size a)
 
 /// Interlude for spec proofs
 /// =====================================
 val update_multi_zero:
-  key_size : key_size_ty ->
+  #a : alg ->
+  key_size : key_size_ty a ->
   i:index ->
-  acc:t ->
+  acc:t a ->
   prevlen:nat{prevlen % Spec.size_block a = 0} ->
   Lemma
-  (requires (prevlen <= max_input_length key_size))
-  (ensures (update_multi_s key_size i acc prevlen S.empty == acc))
+  (requires (prevlen <= max_input_length a key_size))
+  (ensures (update_multi_s #a key_size i acc prevlen S.empty == acc))
 
-let update_multi_zero key_size () acc prevlen =
-  let es = Hash.nat_to_extra_state (to_hash_alg a) (blake2_prevlength key_size prevlen) in
+let update_multi_zero #a key_size () acc prevlen =
+  let es = Hash.nat_to_extra_state (to_hash_alg a) (blake2_prevlength a key_size prevlen) in
   let s = (acc, es) in
   Spec.Hash.Lemmas.update_multi_zero (to_hash_alg a) s
 
 val update_multi_associative:
-  key_size : key_size_ty ->
+  #a : alg ->
+  key_size : key_size_ty a ->
   i:index ->
-  acc: t ->
+  acc: t a ->
   prevlen1:nat ->
   prevlen2:nat ->
   input1:S.seq uint8 ->
@@ -266,7 +265,7 @@ val update_multi_associative:
     prevlen1 % Spec.size_block a = 0 /\
     S.length input1 % Spec.size_block a = 0 /\
     S.length input2 % Spec.size_block a = 0 /\
-    prevlen1 + S.length input1 + S.length input2 <= max_input_length key_size /\
+    prevlen1 + S.length input1 + S.length input2 <= max_input_length a key_size /\
     prevlen2 = prevlen1 + S.length input1))
   (ensures (
     let input = S.append input1 input2 in
@@ -275,8 +274,8 @@ val update_multi_associative:
     update_multi_s key_size i (update_multi_s key_size i acc prevlen1 input1) prevlen2 input2 ==
       update_multi_s key_size i acc prevlen1 input))
 
-let update_multi_associative key_size () acc prevlen1 prevlen2 input1 input2 =
-  let es = Hash.nat_to_extra_state (to_hash_alg a) (blake2_prevlength key_size prevlen1) in
+let update_multi_associative #a key_size () acc prevlen1 prevlen2 input1 input2 =
+  let es = Hash.nat_to_extra_state (to_hash_alg a) (blake2_prevlength a key_size prevlen1) in
   let s = (acc, es) in
   Spec.Hash.Lemmas.update_multi_associative (to_hash_alg a) s input1 input2;
   Spec.Hash.Incremental.Lemmas.update_multi_extra_state_eq (to_hash_alg a) s input1;
@@ -285,11 +284,12 @@ let update_multi_associative key_size () acc prevlen1 prevlen2 input1 input2 =
 /// A helper function: the hash incremental function defined with the functions
 /// locally defined (with a signature adapted to the functor).
 val blake2_hash_incremental_s :
-  #key_size : key_size_ty ->
+  a : alg ->
+  #key_size : key_size_ty a ->
   i:index ->
-  key: I.((k (U32.uint_to_t key_size)).t ()) ->
-  input:S.seq uint8 { S.length input <= max_input_length key_size } ->
-  output:S.seq uint8 { S.length output = output_size }
+  key: I.((k #a (U32.uint_to_t key_size)).t ()) ->
+  input:S.seq uint8 { S.length input <= max_input_length a key_size } ->
+  output:S.seq uint8 { S.length output = output_size a }
 
 let size_block_props (a : Spec.alg) :
   Lemma(
@@ -297,14 +297,14 @@ let size_block_props (a : Spec.alg) :
     Spec.size_block a > 0) = ()
 
 #push-options "--z3cliopt smt.arith.nl=false"
-let blake2_hash_incremental_s #key_size i key input =
+let blake2_hash_incremental_s a #key_size i key input =
   (**) size_block_props a;
   (**) Math.Lemmas.modulo_lemma 0 (Spec.size_block a);
   let bs, l = Spec.Hash.Incremental.split_blocks (to_hash_alg a) input in
-  let acc1 = init_s #key_size i key in
-  let acc2 = update_multi_s key_size i acc1 0 bs in
-  let acc3 = update_last_s key_size i acc2 (S.length bs) l in
-  let acc4 = finish_s #key_size i key acc3 in
+  let acc1 = init_s #a #key_size i key in
+  let acc2 = update_multi_s #a key_size i acc1 0 bs in
+  let acc3 = update_last_s #a key_size i acc2 (S.length bs) l in
+  let acc4 = finish_s #a #key_size i key acc3 in
   acc4
 #pop-options
 
@@ -312,34 +312,36 @@ let blake2_hash_incremental_s #key_size i key input =
 /// with a signature adapted to the functor give the same result, if properly called,
 /// as the original hash incremental functions.
 val blake2_hash_incremental_s_is_hash_incremental :
-  #key_size : key_size_ty ->
+  a : alg ->
+  #key_size : key_size_ty a ->
   i:index ->
-  key: I.((k (U32.uint_to_t key_size)).t ()) ->
-  input:S.seq uint8 { S.length input <= max_input_length key_size } ->
+  key: I.((k #a (U32.uint_to_t key_size)).t ()) ->
+  input:S.seq uint8 { S.length input <= max_input_length a key_size } ->
   Lemma(
-    blake2_hash_incremental_s #key_size i key input ==
+    blake2_hash_incremental_s a #key_size i key input ==
       Spec.Hash.Incremental.blake2_hash_incremental (to_hash_alg a) key_size key input)
 
 let init_s_blake2_init_eq
-  (#key_size : key_size_ty)
+  (a : alg)
+  (#key_size : key_size_ty a)
   (i:index)
-  (key: I.((k (U32.uint_to_t key_size)).t ())) :
+  (key: I.((k #a (U32.uint_to_t key_size)).t ())) :
   Lemma(
-    (init_s #key_size i key,
-     Hash.nat_to_extra_state (to_hash_alg a) (blake2_prevlength key_size 0)) ==
+    (init_s #a #key_size i key,
+     Hash.nat_to_extra_state (to_hash_alg a) (blake2_prevlength a key_size 0)) ==
       Spec.Hash.Incremental.blake2_init (to_hash_alg a) key_size key) =
   ()
 
 #push-options "--z3cliopt smt.arith.nl=false"
-let blake2_hash_incremental_s_is_hash_incremental #key_size i key input =
+let blake2_hash_incremental_s_is_hash_incremental a #key_size i key input =
   size_block_props a;
   Math.Lemmas.modulo_lemma 0 (Spec.size_block a);
   let bs, l = Spec.Hash.Incremental.split_blocks (to_hash_alg a) input in
-  let acc1 = init_s #key_size i key in
+  let acc1 = init_s #a #key_size i key in
   let acc2 = update_multi_s key_size i acc1 0 bs in
   let acc3 = update_last_s key_size i acc2 (S.length bs) l in
-  let acc4 = finish_s #key_size i key acc3 in
-  assert(acc4 == blake2_hash_incremental_s #key_size i key input); (* sanity check *)
+  let acc4 = finish_s #a #key_size i key acc3 in
+  assert(acc4 == blake2_hash_incremental_s a #key_size i key input); (* sanity check *)
   let s1 = Spec.Hash.Incremental.blake2_init (to_hash_alg a) key_size key in
   let s2 = Agile.update_multi (to_hash_alg a) s1 bs in
   let prevlen = S.length bs in (* dummy value: this variable is actually not used *)
@@ -349,18 +351,18 @@ let blake2_hash_incremental_s_is_hash_incremental #key_size i key input =
   assert(s4 == s4'); (* sanity check *)
   (* The proof *)
   (* 1 *)
-  let es1 = Hash.nat_to_extra_state (to_hash_alg a) (blake2_prevlength key_size 0) in
+  let es1 = Hash.nat_to_extra_state (to_hash_alg a) (blake2_prevlength a key_size 0) in
   let s1' = (acc1, es1) in
-  init_s_blake2_init_eq i key;
+  init_s_blake2_init_eq a i key;
   assert(s1' == s1);
   (* 2 *)
   Spec.Hash.Incremental.Lemmas.update_multi_extra_state_eq (to_hash_alg a) s1 bs;
   Spec.Hash.Lemmas.extra_state_add_nat_bound_lem2 #(to_hash_alg a) es1 (S.length bs);
-  let es2 = Hash.nat_to_extra_state (to_hash_alg a) (blake2_prevlength key_size (S.length bs)) in
+  let es2 = Hash.nat_to_extra_state (to_hash_alg a) (blake2_prevlength a key_size (S.length bs)) in
   let s2' = (acc2, es2) in
-  blake2_prevlength_add_right_eq key_size 0 (S.length bs);
+  blake2_prevlength_add_right_eq a key_size 0 (S.length bs);
   add_zero_left_is_same (S.length bs);
-  assert(blake2_prevlength key_size 0 + S.length bs = blake2_prevlength key_size (S.length bs));
+  assert(blake2_prevlength a key_size 0 + S.length bs = blake2_prevlength a key_size (S.length bs));
   assert(s2' == s2);
   (* 3 *)
   let es3 = Hash.nat_to_extra_state (to_hash_alg a) 0 in
@@ -371,42 +373,44 @@ let blake2_hash_incremental_s_is_hash_incremental #key_size i key input =
 #pop-options
 
 val spec_is_incremental:
-  #key_size : key_size_ty ->
+  a : alg ->
+  #key_size : key_size_ty a ->
   i:index ->
-  key: I.((k (U32.uint_to_t key_size)).t ()) ->
-  input:S.seq uint8 { S.length input <= max_input_length key_size } ->
+  key: I.((k #a (U32.uint_to_t key_size)).t ()) ->
+  input:S.seq uint8 { S.length input <= max_input_length a key_size } ->
   Lemma (
     let bs, l = Spec.Hash.Incremental.split_blocks (to_hash_alg a) input in
-    let hash0 = init_s #key_size i key in
+    let hash0 = init_s #a #key_size i key in
     let hash1 = update_multi_s key_size i hash0 0 bs in
     let hash2 = update_last_s key_size i hash1 (S.length bs) l in
-    finish_s #key_size i key hash2 `S.equal` (spec_s #key_size) i key input)
+    finish_s #a #key_size i key hash2 `S.equal` (spec_s a #key_size) i key input)
 
-let spec_is_incremental #key_size i key input =
-  blake2_hash_incremental_s_is_hash_incremental i key input;
+let spec_is_incremental a #key_size i key input =
+  blake2_hash_incremental_s_is_hash_incremental a i key input;
   Spec.Hash.Incremental.blake2_is_hash_incremental (to_hash_alg a) key_size key input
 
 val update_multi_eq :
-  key_size : key_size_ty ->
+  #a : alg ->
+  key_size : key_size_ty a ->
   nb : nat ->
-  acc : t ->
+  acc : t a ->
   prevlen : nat {prevlen % Spec.size_block a = 0 } ->
   blocks : S.seq uint8 ->
   Lemma
     (requires (
-      prevlen + S.length blocks <= max_input_length key_size /\
-      blake2_prevlength key_size prevlen + S.length blocks <= Hash.max_extra_state (to_hash_alg a) /\
+      prevlen + S.length blocks <= max_input_length a key_size /\
+      blake2_prevlength a key_size prevlen + S.length blocks <= Hash.max_extra_state (to_hash_alg a) /\
       S.length blocks = Hash.block_length (to_hash_alg a) * nb))
     (ensures (
-      let prevlen' = blake2_prevlength key_size prevlen in
+      let prevlen' = blake2_prevlength a key_size prevlen in
       update_multi_s key_size () acc prevlen blocks ==
         Loops.repeati #(Hash.words_state' (to_hash_alg a)) nb
                        (Spec.blake2_update1 a prevlen' blocks) acc))
 
-let update_multi_eq key_size nb acc prevlen blocks =
+let update_multi_eq #a key_size nb acc prevlen blocks =
   let blocks', _ = Seq.split blocks (nb * Hash.block_length (to_hash_alg a)) in
   assert(blocks' `Seq.equal` blocks);
-  let prevlen' = blake2_prevlength key_size prevlen in
+  let prevlen' = blake2_prevlength a key_size prevlen in
   let es = Hash.nat_to_extra_state (to_hash_alg a) prevlen' in
   Spec.Hash.Incremental.repeati_blake2_update1_is_update_multi (to_hash_alg a)
                                                                nb prevlen'
@@ -417,20 +421,21 @@ let update_multi_eq key_size nb acc prevlen blocks =
     Hash.extra_state_add_nat #(to_hash_alg a) es (S.length blocks))
 
 val update_last_eq :
-  key_size : key_size_ty ->
+  #a : alg ->
+  key_size : key_size_ty a ->
   prevlen : nat{prevlen % Hash.block_length (to_hash_alg a) = 0} ->
   last : S.seq uint8 {S.length last <= Hash.block_length (to_hash_alg a) /\
-                      prevlen + S.length last <= max_input_length key_size} ->
-  acc : t ->
+                      prevlen + S.length last <= max_input_length a key_size} ->
+  acc : t a ->
   Lemma
   (ensures (
-    let prevlen' = blake2_prevlength key_size prevlen in
+    let prevlen' = blake2_prevlength a key_size prevlen in
     Spec.blake2_update_last a prevlen' (S.length last) last acc ==
       update_last_s key_size () acc prevlen last))
 
-let update_last_eq key_size prevlen last acc =
+let update_last_eq #a key_size prevlen last acc =
   (* Checking how to unfold the ``update_last_s`` definition *)
-  let prevlen' = blake2_prevlength key_size prevlen in
+  let prevlen' = blake2_prevlength a key_size prevlen in
   let es = Hash.nat_to_extra_state (to_hash_alg a) prevlen' in
   let s = acc, es in
   let s' = Spec.Hash.Incremental.update_last_blake (to_hash_alg a) s prevlen' last in
@@ -452,51 +457,73 @@ let update_last_eq key_size prevlen last acc =
   assert(Hash.extra_state_v (Hash.extra_state_add_nat es (S.length last)) ==
          Hash.extra_state_v es + S.length last)
 
+/// TODO: duplicate with Spec.Hash.Incremental.fst - MOVE
 /// Equality between the state types defined by blake2s and the generic hash.
 /// The equality is not trivial because of subtleties linked to the way types are
 /// encoded for Z3.
-val state_types_equalities : unit ->
+val state_types_equalities : (a : alg) ->
   Lemma(Spec.Blake2.state a == Hash.words_state' (to_hash_alg a))
 
-let state_types_equalities () =
+let state_types_equalities a =
   let open Lib.Sequence in
   let open Lib.IntTypes in
-  assert(Spec.Blake2.state a == lseq (Spec.row a) 4);
-  assert_norm(Hash.words_state' (to_hash_alg a) == m:Seq.seq (Spec.row a) {Seq.length m = 4});
-  assert_norm(lseq (Spec.row a) 4 == m:Seq.seq (Spec.row a) {Seq.length m == 4});
-  assert(lseq (Spec.row a) 4 == m:Seq.seq (Spec.row a) {Seq.length m = 4})
+  (* Because of the necessity to be able to normalize, we basically do
+   * the same proof twice. TODO: find a better way *)
+  match a with
+  | Spec.Blake2S ->
+    let a = Spec.Blake2S in (* small trick to get a proper normalization *)
+    let row = Spec.row a in
+    assert(Spec.state a == lseq row 4);
+    assert_norm(Hash.words_state' (to_hash_alg a) == m:Seq.seq row {Seq.length m = 4});
+    assert_norm(lseq row 4 == m:Seq.seq row {Seq.length m == 4});
+    assert(lseq row 4 == m:Seq.seq row {Seq.length m = 4})
+  | Spec.Blake2B ->
+    let a = Spec.Blake2B in
+    let row = Spec.row a in
+    assert(Spec.state a == lseq row 4);
+    assert_norm(Hash.words_state' (to_hash_alg a) == m:Seq.seq row {Seq.length m = 4});
+    assert_norm(lseq row 4 == m:Seq.seq row {Seq.length m == 4});
+    assert(lseq row 4 == m:Seq.seq row {Seq.length m = 4})
 
 (* TODO: find a way not to duplicate the block spec *)
-val update_multi:
-  key_len : key_size_t ->
+inline_for_extraction noextract
+val mk_update_multi:
+  a : alg ->
+  m : m_spec ->
+  key_len : key_size_t a ->
   (i:G.erased index -> (
   let i = G.reveal i in
-  s:s ->
-  prevlen:U64.t { U64.v prevlen % U32.v (block_len) = 0 } ->
-  blocks:B.buffer uint8 { B.length blocks % U32.v (block_len) = 0 } ->
+  s:s a m ->
+  prevlen:U64.t { U64.v prevlen % U32.v (block_len a) = 0 } ->
+  blocks:B.buffer uint8 { B.length blocks % U32.v (block_len a) = 0 } ->
   len: U32.t { U32.v len = B.length blocks /\
-               U64.v prevlen + U32.v len <= max_input_length (U32.v key_len) } ->
+               U64.v prevlen + U32.v len <= max_input_length a (U32.v key_len) } ->
   ST.Stack unit
   (requires fun h0 ->
-    let state = stateful_blake2s_32 in
+    let state = stateful_blake2 a m in
     state.I.invariant #i h0 s /\
     B.live h0 blocks /\
     B.(loc_disjoint (state.I.footprint #i h0 s) (loc_buffer blocks)))
   (ensures fun h0 _ h1 ->
-    let state = stateful_blake2s_32 in
+    let state = stateful_blake2 a m in
     B.(modifies (state.I.footprint #i h0 s) h0 h1) /\
     state.I.footprint #i h0 s == state.I.footprint #i h1 s /\
     state.I.invariant #i h1 s /\
-    state.I.v i h1 s == update_multi_s (U32.v key_len) i (state.I.v i h0 s) (U64.v prevlen)
+    state.I.v i h1 s == update_multi_s #a (U32.v key_len) i (state.I.v i h0 s) (U64.v prevlen)
                                                   (B.as_seq h0 blocks) /\
     (state.I.freeable #i h0 s ==> state.I.freeable #i h1 s))))
 
-let update_multi key_len i acc prevlen blocks len =
+#push-options "--z3cliopt smt.arith.nl=false"
+let mk_update_multi a m key_len i acc prevlen blocks len =
+  (**) size_block_props a;
   [@inline_let] let wv = get_wv acc in
   [@inline_let] let h = get_state_p acc in
   (**) let h0 = ST.get () in
-  let nb = U32.(len /^ block_len) in
-  [@inline_let] let prevlen' = blake2_prevlen key_len prevlen in
+  let nb = U32.(len /^ block_len a) in
+  (**) Math.Lemmas.div_exact_r (U32.v len) (U32.v (block_len a));
+  (**) Math.Lemmas.multiply_fractions (U32.v len) (U32.v (block_len a));
+  [@inline_let] let prevlen' = blake2_prevlen a key_len prevlen in
+  (**) assert(Lib.Buffer.disjoint wv h);
   Impl.blake2_update_multi #a #m #len (Impl.blake2_update_block #a #m) wv h
                            prevlen' blocks nb;
   (**) let h3 = ST.get () in
@@ -505,53 +532,59 @@ let update_multi key_len i acc prevlen blocks len =
   (**)                  (Spec.blake2_update1 a (Lib.IntTypes.uint_v prevlen')
   (**)                                       (B.as_seq h0 blocks))
   (**)                  (s_v h0 acc));
-  (**) state_types_equalities ();
+  (**) state_types_equalities a;
   (**) assert(Spec.Blake2.state a == Hash.words_state' (to_hash_alg a));
   (**) update_multi_eq (U32.v key_len) (U32.v nb) (s_v h0 acc) (U64.v prevlen) (B.as_seq h0 blocks);
-  (**) assert(Lib.IntTypes.uint_v prevlen' = blake2_prevlength (U32.v key_len) (U64.v prevlen));
+  (**) assert(Lib.IntTypes.uint_v prevlen' = blake2_prevlength a (U32.v key_len) (U64.v prevlen));
   (**) assert(s_v h3 acc == update_multi_s (U32.v key_len) () (s_v h0 acc) (U64.v prevlen) (B.as_seq h0 blocks));
-  (**) assert(B.(modifies (stateful_blake2s_32.I.footprint #() h0 acc) h0 h3))
+  (**) assert(B.(modifies ((stateful_blake2 a m).I.footprint #() h0 acc) h0 h3))
+#pop-options
 
-val update_last:
-  key_len : key_size_t ->
+inline_for_extraction noextract
+val mk_update_last:
+  a : alg ->
+  m : m_spec ->
+  key_len : key_size_t a ->
   (i: G.erased index -> (
   let i = G.reveal i in
-  s:s ->
-  prevlen:U64.t { U64.v prevlen % U32.v (block_len) = 0 } ->
+  s:s a m ->
+  prevlen:U64.t { U64.v prevlen % U32.v (block_len a) = 0 } ->
   last:B.buffer uint8 ->
   last_len:U32.t{
     last_len = B.len last /\
-    U32.v last_len <= U32.v (block_len) /\
-    U64.v prevlen + U32.v last_len <= max_input_length (U32.v key_len)} ->
+    U32.v last_len <= U32.v (block_len a) /\
+    U64.v prevlen + U32.v last_len <= max_input_length a (U32.v key_len)} ->
   ST.Stack unit
   (requires fun h0 ->
-    let state = stateful_blake2s_32 in
+    let state = stateful_blake2 a m in
     state.I.invariant #i h0 s /\
     B.live h0 last /\
     B.(loc_disjoint (state.I.footprint #i h0 s) (loc_buffer last)))
   (ensures fun h0 _ h1 ->
-    let state = stateful_blake2s_32 in
+    let state = stateful_blake2 a m in
     state.I.invariant #i h1 s /\
-    state.I.v i h1 s == update_last_s (U32.v key_len) i (state.I.v i h0 s)
+    state.I.v i h1 s == update_last_s #a (U32.v key_len) i (state.I.v i h0 s)
                                       (U64.v prevlen) (B.as_seq h0 last) /\
     B.(modifies (state.I.footprint #i h0 s) h0 h1) /\
     state.I.footprint #i h0 s == state.I.footprint #i h1 s /\
     (state.I.freeable #i h0 s ==> state.I.freeable #i h1 s))))
 
-let update_last key_len i acc prevlen last last_len =
+#push-options "--ifuel 1 --z3cliopt smt.arith.nl=false"
+let mk_update_last a m key_len i acc prevlen last last_len =
+  (**) size_block_props a;
   [@inline_let] let wv = get_wv acc in
   [@inline_let] let h = get_state_p acc in
   (**) let h0 = ST.get () in
   (**) assert_norm(U64.v prevlen + U32.v last_len <= Spec.Blake2.max_limb a);
   [@inline_let]
-  let prevlen' = blake2_prevlen key_len prevlen in
-  assert((U64.v prevlen) % Hash.block_length (to_hash_alg a) = 0);
-  assert(B.length last <= Hash.block_length (to_hash_alg a));
-  assert(U64.v prevlen + B.length last <= max_input_length (U32.v key_len));
-  (* SH: this call loops if moved at the end of the proof *)
-  (**) update_last_eq (U32.v key_len) (U64.v prevlen) (B.as_seq h0 last) (s_v h0 acc);
+  let prevlen' = blake2_prevlen a key_len prevlen in
+  (**) assert((U64.v prevlen) % Hash.block_length (to_hash_alg a) = 0);
+  (**) assert(B.length last <= Hash.block_length (to_hash_alg a));
+  (**) assert(U64.v prevlen + B.length last <= max_input_length a (U32.v key_len));
   Impl.blake2_update_last #a #m (Impl.blake2_update_block #a #m) #last_len
                           wv h prevlen' last_len last;
+  (* SH: if not put at the proper place, this call makes the proof loop or randomly fail *)
+  (**) update_last_eq (U32.v key_len) (U64.v prevlen) (B.as_seq h0 last) (s_v h0 acc);
   (**) let h2 = ST.get () in
   (**) assert(
   (**)   Core.state_v h2 h ==
@@ -560,61 +593,67 @@ let update_last key_len i acc prevlen last last_len =
   (**)                               (Core.state_v h0 h));
   (**) assert(s_v h2 acc ==
   (**)   update_last_s (U32.v key_len) () (s_v h0 acc) (U64.v prevlen) (B.as_seq h0 last))
+#pop-options
 
 #push-options "--ifuel 1"
 inline_for_extraction noextract
-let blake2s_32 (key_len : key_size_t) : I.block unit =
+let blake2 (a : alg) (m : m_spec) (key_len : key_size_t a) //: I.block unit =
+  =
   I.Block
     I.Erased (* key management *)
     
-    stateful_blake2s_32 (* state *)
+    (stateful_blake2 a m) (* state *)
     (k key_len) (* key *)
     
-    (fun () -> max_input_length (Spec.max_key a)) (* max_input_length *)
-    (fun () -> output_len) (* output_len *)
-    (fun () -> block_len) (* block_len *)
+    (fun () -> max_input_length a (Spec.max_key a)) (* max_input_length *)
+    (fun () -> output_len a) (* output_len *)
+    (fun () -> block_len a) (* block_len *)
     
-    (fun () k -> init_s #(U32.v key_len) () k) (* init_s *)
+    (fun () k -> init_s #a #(U32.v key_len) () k) (* init_s *)
     (fun () acc prevlen input -> update_multi_s (U32.v key_len) () acc prevlen input) (* update_multi_s *)
     (fun () acc prevlen input -> update_last_s (U32.v key_len) () acc prevlen input) (* update_last_s *)
-    (fun () k acc -> finish_s #(U32.v key_len) () k acc) (* finish_s *)
-    (fun () -> spec_s #(U32.v key_len) ()) (* spec_s *)
+    (fun () k acc -> finish_s #a #(U32.v key_len) () k acc) (* finish_s *)
+    (fun () -> spec_s a #(U32.v key_len) ()) (* spec_s *)
 
     (fun () prevlen acc -> update_multi_zero (U32.v key_len) () prevlen acc) (* update_multi_zero *)
     (* update_multi_associative *)
     (fun () acc prevlen1 prevlen2 input1 input2 ->
       update_multi_associative (U32.v key_len) () acc prevlen1 prevlen2 input1 input2)
-    (fun () k input -> spec_is_incremental #(U32.v key_len) () k input) (* spec_is_incremental *)
+    (fun () k input -> spec_is_incremental a #(U32.v key_len) () k input) (* spec_is_incremental *)
     (fun _ acc -> ()) (* index_of_state *)
 
     (* init *)
     (fun _ key acc ->
       [@inline_let] let wv = get_wv acc in
       [@inline_let] let h = get_state_p acc in
-      Impl.blake2_init #a #m (Impl.blake2_update_block #a #m) wv h key_len key output_len)
+      Impl.blake2_init #a #m (Impl.blake2_update_block #a #m) wv h key_len key (output_len a))
 
     (* update_multi *)
-    (fun _ acc prevlen blocks len -> update_multi key_len () acc prevlen blocks len)
+    (fun _ acc prevlen blocks len -> mk_update_multi a m key_len () acc prevlen blocks len)
 
     (* update_last *)
     (fun _ acc prevlen last last_len ->
-      update_last key_len () acc prevlen last last_len)
+      mk_update_last a m key_len () acc prevlen last last_len)
 
     (* finish *)
     (fun _ k acc dst ->
       [@inline_let] let wv = get_wv acc in
       [@inline_let] let h = get_state_p acc in
-      Impl.blake2_finish #a #m output_len dst h)
+      Impl.blake2_finish #a #m (output_len a) dst h)
 #pop-options
 
 /// The incremental hash functions instantiations
-let create_in (key_len : key_size_t) =
-  F.create_in (blake2s_32 key_len) () s (I.optional_key () I.Erased (k key_len))
-let init (key_len : key_size_t) =
-  F.init (blake2s_32 key_len) (G.hide ()) s (I.optional_key () I.Erased (k key_len))
-let update (key_len : key_size_t) =
-  F.update (blake2s_32 key_len) (G.hide ()) s (I.optional_key () I.Erased (k key_len))
-let finish (key_len : key_size_t) =
-  F.mk_finish (blake2s_32 key_len) () s (I.optional_key () I.Erased (k key_len))
-let free (key_len : key_size_t) =
-  F.free (blake2s_32 key_len) (G.hide ()) s (I.optional_key () I.Erased (k key_len))
+let mk_create_in (a : alg) (m : m_spec) (key_len : key_size_t a) =
+  F.create_in (blake2 a m key_len) () (s a m) (I.optional_key () I.Erased (k key_len))
+
+let mk_init (a : alg) (m : m_spec) (key_len : key_size_t a) =
+  F.init (blake2 a m key_len) (G.hide ()) (s a m) (I.optional_key () I.Erased (k key_len))
+
+let mk_update (a : alg) (m : m_spec) (key_len : key_size_t a) =
+  F.update (blake2 a m key_len) (G.hide ()) (s a m) (I.optional_key () I.Erased (k key_len))
+
+let mk_finish (a : alg) (m : m_spec) (key_len : key_size_t a) =
+  F.mk_finish (blake2 a m key_len) () (s a m) (I.optional_key () I.Erased (k key_len))
+
+let mk_free (a : alg) (m : m_spec) (key_len : key_size_t a) =
+  F.free (blake2 a m key_len) (G.hide ()) (s a m) (I.optional_key () I.Erased (k key_len))
